## 설명
내가 만든 안드로이드 리버싱 문제 간단한 거임 

## 문제

((a + b + c) - (a + e)) ^ f - g ^ h == -125
(h + u - t) + (d ^ k) + k + l == 314
m + n + p + q - s - t - r + i + k == 390
a + b - c + e + d - k + i - m - n == 189
a + b + c + d + e + f + g + h + i + j + k + l == 1074
m + n + o + p +q + r + s + t +u == 841
(a + b) ^ (c + d) == 13
(e + f) ^ (g + h) == 114
(i + j) ^ (k + l) == 79
(m + n) ^ (o + p) == 10
(q + r) ^ (s + t + u) == 81
b * c - d * f == -3015
(a + q) ^ (d + o) == 88
(i - j) ^ (m + n)==216
b * u * n - e * k * s == 988494
s * 3 - 2 == b
s + a + b + c + d + e == 465
